WIP

Foundation/Modal/Neighborhood/Completeness.lean
@@ -1,5 +1,138 @@
 import Foundation.Modal.MaximalConsistentSet
+import Foundation.Modal.Neighborhood.Basic
 
 namespace LO.Modal
+
+open LO.Entailment
+
+
+section
+
+variable {α : Type*} [DecidableEq α]
+variable {S} [Entailment (Formula α) S]
+variable {𝓢 : S} [Entailment.Cl 𝓢]
+
+def MaximalConsistentSet.proofset (𝓢 : S) (φ : Formula α) : Set (MaximalConsistentSet 𝓢) := { Γ : MaximalConsistentSet 𝓢 | φ ∈ Γ }
+
+namespace MaximalConsistentSet.proofset
+
+local notation "‖" φ "‖" => MaximalConsistentSet.proofset 𝓢 φ
+
+variable {φ ψ : Formula α}
+
+lemma eq_top : ‖⊤‖ = Set.univ := by simp [proofset];
+
+lemma eq_bot : ‖⊥‖ = ∅ := by simp [proofset];
+
+lemma eq_neg : ‖∼φ‖ = ‖φ‖ᶜ := by simp [proofset]; tauto;
+
+lemma eq_imp : ‖φ ➝ ψ‖ = (‖φ‖ᶜ ∪ ‖ψ‖) := by
+  ext;
+  simp [proofset];
+  tauto;
+
+lemma eq_and : ‖φ ⋏ ψ‖ = ‖φ‖ ∩ ‖ψ‖ := by simp [proofset]; tauto;
+
+lemma eq_or : ‖φ ⋎ ψ‖ = ‖φ‖ ∪ ‖ψ‖ := by simp [proofset]; tauto;
+
+attribute [simp, grind]
+  eq_top
+  eq_bot
+  eq_neg
+  eq_imp
+  eq_and
+  eq_or
+
+@[grind]
+lemma imp_subset : 𝓢 ⊢! φ ➝ ψ ↔ ‖φ‖ ⊆ ‖ψ‖ := by
+  constructor;
+  . intro h Γ;
+    apply iff_mem_imp.mp $ iff_forall_mem_provable.mpr h Γ;
+  . intro h;
+    apply iff_forall_mem_provable.mp;
+    intro Γ;
+    apply iff_mem_imp.mpr $ @h Γ;
+
+@[grind]
+lemma iff_subset : 𝓢 ⊢! φ ⭤ ψ ↔ ‖φ‖ = ‖ψ‖ := by
+  constructor;
+  . intro h;
+    apply Set.eq_of_subset_of_subset <;>
+    . apply imp_subset.mp;
+      cl_prover [h];
+  . intro h;
+    have ⟨h₁, h₂⟩ := Set.Subset.antisymm_iff.mp h;
+    replace h₁ := imp_subset.mpr h₁;
+    replace h₂ := imp_subset.mpr h₂;
+    cl_prover [h₁, h₂];
+
+end MaximalConsistentSet.proofset
+
+end
+
+
+section
+
+variable {S} [Entailment (Formula ℕ) S]
+variable {𝓢 : S} [Entailment.Cl 𝓢]
+
+namespace Neighborhood
+
+open Formula (atom)
+open Formula.Neighborhood
+open MaximalConsistentSet
+
+variable {φ ψ ξ : Formula ℕ}
+
+class Frame.IsCanonical (𝓢 : S) (F : Frame) where
+  def_equiv : F.World = (MaximalConsistentSet 𝓢)
+  def_ℬ : ∀ φ, (F.ℬ (def_equiv ▸ (proofset 𝓢 φ))) = (def_equiv ▸ proofset 𝓢 (□φ))
+
+variable {F : Frame} [canonical : F.IsCanonical 𝓢]
+
+abbrev canonicalModel (𝓢 : S) (F : Frame) [canonical : F.IsCanonical 𝓢] : Model where
+  toFrame := F
+  Val a := canonical.def_equiv ▸ proofset 𝓢 (.atom a)
+
+instance : Coe (Set (MaximalConsistentSet 𝓢)) (Set (canonicalModel 𝓢 F).World) := ⟨λ Γ => canonical.def_equiv ▸ Γ⟩
+
+@[reducible]
+instance : Semantics (Formula ℕ) (canonicalModel 𝓢 F).World := Formula.Neighborhood.Satisfies.semantics (M := canonicalModel 𝓢 F)
+
+set_option pp.proofs true
+
+lemma truthlemma : ↑(proofset 𝓢 φ) = ((canonicalModel 𝓢 F).truthset φ) := by
+  induction φ with
+  | hatom => simp
+  | hfalsum =>
+    sorry;
+  | himp φ ψ ihφ ihψ =>
+    simp_all [MaximalConsistentSet.proofset.eq_imp, ←ihφ, ←ihψ];
+    sorry;
+  | hbox φ ihφ =>
+    rw [Model.truthset.eq_box, ←ihφ, canonical.def_ℬ];
+
+lemma complete_of_canonical_frame
+  (C : FrameClass)
+  (F : Frame) [F_canonical : F.IsCanonical 𝓢] (hFC : F ∈ C)
+  : LO.Complete 𝓢 C := by
+  constructor;
+  intro φ;
+  contrapose!;
+  intro hφ;
+  have := FormulaSet.unprovable_iff_singleton_neg_consistent.mpr hφ;
+  obtain ⟨Γ, hΓ⟩ := lindenbaum this;
+  apply not_validOnFrameClass_of_exists_model_world;
+  use (canonicalModel 𝓢 F), (F_canonical.def_equiv ▸ Γ);
+  constructor;
+  . apply hFC;
+  . simp only [Semantics.Realize, Satisfies, ←truthlemma];
+    suffices Γ ∉ proofset 𝓢 φ by
+      sorry;
+    simpa [proofset, ←iff_mem_neg] using hΓ;
+
+end Neighborhood
+
+end
 
 end LO.Modal
